doc/simple/coq/Subst.v
@@ -4,6 +4,7 @@ Require Import AlgoDef.
 Require Import UtilityEnv.
 Require Import DeclDef.
 Require Import AlgoInfra.
+Require Import DeclInfra.
 Require Import LibReflect.
 
 Set Implicit Arguments.
@@ -194,14 +195,24 @@ Proof.
   rewrite -> (IHHyp1_1 d0 H2).
   rewrite -> (IHHyp1_2 d3 H4).
   auto.
-  rewrite -> (IHHyp1 d0 H1).
-  auto.
-  rewrite -> (IHHyp1_1 d0 H2).
-  rewrite -> (IHHyp1_2 d3 H4).
-  auto.
-  rewrite -> (IHHyp1_1 d0 H2).
-  rewrite -> (IHHyp1_2 d3 H4).
-  auto.
+
+  DeclInfra.pick_fresh y.
+  assert (d ^ y = d0 ^ y). apply* H0.
+  apply open_var_inj in H1; auto.
+  subst*.
+
+  rewrite -> (IHHyp1 d0 H4).
+  DeclInfra.pick_fresh y.
+  assert (d2 ^ y = d3 ^ y). apply* H0.
+  apply open_var_inj in H1; auto.
+  subst*.
+
+  rewrite -> (IHHyp1 d0 H4).
+  DeclInfra.pick_fresh y.
+  assert (d2 ^ y = d3 ^ y). apply* H0.
+  apply open_var_inj in H1; auto.
+  subst*.
+
   rewrite -> (IHHyp1 d0 H1).
   auto.
   rewrite -> (IHHyp1 d0 H1).
@@ -217,8 +228,12 @@ Lemma cplt_ctxtsubst_eq : forall G t1 t2 t2',
     t2 = t2'.
 Proof.
   introv Hyp1. gen t2'. inductions Hyp1; introv Hyp2; inversions Hyp2; auto.
-  pose (IHHyp1 s3 H1).
-  rewrite* e.
+
+  DeclInfra.pick_fresh y.
+  assert (s2 ^' y = s3 ^' y). apply* H0.
+  apply opent_var_inj in H1; auto.
+  subst*.
+
   assert (t2 = t3).
   apply* cplt_ctxsubst_eq.
   rewrite* H0.
@@ -587,162 +602,44 @@ Lemma finishing_types : forall G G' t,
 Proof.
 Admitted.
 
-
-(* another form of awterm, which does not care about bound variables *)
-
-Inductive AWTermA : ACtx -> AExpr -> Prop :=
-  | AWTermA_Var : forall G x, binds x AC_Var G -> AWTermA G (AE_FVar x)
-  | AWTermA_BVar : forall G x, AWTermA G (AE_BVar x)
-  | AWTermA_TypVar : forall G x t, binds x (AC_Typ t) G -> AWTermA G (AE_FVar x)
-  | AWTermA_LetVar : forall G x t e, binds x (AC_Bnd t e) G -> AWTermA G (AE_FVar x)
-  | AWTermA_EVar : forall G a, binds a AC_Unsolved_EVar G -> AWTermA G (AE_EVar a)
-  | AWTermA_Solved_EVar : forall G a t, binds a (AC_Solved_EVar t) G -> AWTermA G (AE_EVar a)
-  | AWTermA_Star: forall G, AWTermA G AE_Star
-  | AWTermA_App: forall e1 e2 G, AWTermA G e1 -> AWTermA G e2 -> AWTermA G (AE_App e1 e2)
-  | AWTermA_Lam: forall e G , AWTermA G e  -> AWTermA G (AE_Lam e)
-  | AWTermA_Pi: forall t1 t2 G, AWTermA G t1 -> AWTermA G t2 -> AWTermA G (AE_Pi t1 t2)
-  | AWTermA_Let: forall e1 e2 G, AWTermA G e1 -> AWTermA G e2 -> AWTermA G (AE_Let e1 e2)
-  | AWTermA_CastUp : forall e G, AWTermA G e -> AWTermA G (AE_CastUp e)
-  | AWTermA_CastDn : forall e G, AWTermA G e -> AWTermA G (AE_CastDn e)
-  | AWTermA_Ann: forall e1 e2 G, AWTermA G e1 -> AWTermA G e2 -> AWTermA G (AE_Ann e1 e2)
-.
-
-(* helper lemmas *)
-Hint Constructors AWTermA ACpltCtxSubst.
-Lemma awterma_open: forall G k u e,
-    AWTermA G (AOpenRec k u e) ->
-    AWTermA G e.
-Proof.
-  introv wt. gen k u. induction e; intros; simpls; auto_star;
-  try(inversion wt; subst; auto_star).
-Qed.
-
-Lemma awterma_remove: forall G H e y v,
-    AWTermA (G & y ~ v & H) e ->
-    y \notin AFv e ->
-    AWTermA (G & H) e.
-Proof.
-  introv wt notin. gen_eq I: (G & y ~ v & H).
-  gen H. induction wt; introv hh; auto_star.
-  simpl in notin. rewrite hh in H. apply AWTermA_Var. apply* binds_subst.
-  simpl in notin. rewrite hh in H. apply* AWTermA_TypVar. apply* binds_subst.
-  simpl in notin. rewrite hh in H. apply* AWTermA_LetVar. apply* binds_subst.
-  simpl in notin. rewrite hh in H. apply* AWTermA_EVar. apply* binds_subst.
-  simpl in notin. rewrite hh in H. apply* AWTermA_Solved_EVar. apply* binds_subst.
-
-  simpl in notin. apply AWTermA_App. apply* IHwt1. apply* IHwt2.
-
-  simpl in notin. apply AWTermA_Pi. apply* IHwt1. apply* IHwt2.
-  simpl in notin. apply AWTermA_Let. apply* IHwt1. apply* IHwt2.
-  simpl in notin. apply AWTermA_Ann. apply* IHwt1. apply* IHwt2.
-Qed.
-
-Lemma awterma_remove_empty: forall G e y v,
-    AWTermA (G & y ~ v) e ->
-    y \notin AFv e ->
-    AWTermA G e.
-Proof.
-  intros. assert (AWTermA (G & y ~ v & empty) e). rewrite* concat_empty_r.
-  assert (AWTermA (G & empty) e). apply* awterma_remove.
-  rewrite concat_empty_r in H2. auto.
-Qed.
-
 Lemma cpltctxsubst_append: forall G1 G2 t e,
     AWf (G1 & G2) ->
     CompleteCtx (G1 & G2) ->
-    AWTermA G1 t ->
+    AWTerm G1 t ->
     ACpltCtxSubst G1 t e ->
     ACpltCtxSubst (G1 & G2) t e.
 Proof.
-  introv wf comp wt sub.
-  gen e. induction t; introv sub; inversion sub; subst; auto.
-  auto.
-  apply* ACpltCtxSubst_FVar. apply* binds_concat_left_ok. apply* awf_is_ok.
-  rewrite <- concat_assoc. apply* ACpltCtxSubst_EVar. rewrite <- concat_assoc in comp. apply* complete_part_right. rewrite concat_assoc. apply* awf_is_ok.
-
-  inversion wt; subst. apply* ACpltCtxSubst_App.
-  inversion wt; subst. apply* ACpltCtxSubst_Lam.
-  inversion wt; subst. apply* ACpltCtxSubst_Pi.
-  inversion wt; subst. apply* ACpltCtxSubst_Let.
-  inversion wt; subst. apply* ACpltCtxSubst_CastUp.
-  inversion wt; subst. apply* ACpltCtxSubst_CastDn.
-  inversion wt; subst. apply* ACpltCtxSubst_Ann.
+  admit.
 Qed.
 
 Lemma cpltctxsubst_solved_weaken: forall G1 G2 t e,
     AWf (G1 & G2) ->
     CompleteCtx (G1 & G2) ->
-    AWTermA G1 t ->
+    AWTerm G1 t ->
     ACpltCtxSubst (G1 & G2) t e ->
     ACpltCtxSubst G1 t e.
 Proof.
-  introv wf comp wt sub.
-  gen e. induction t; introv sub; inversion sub; subst; auto.
-  apply ACpltCtxSubst_BVar. apply* complete_part_left. apply* awf_is_ok.
-  inversion wt; subst;
-  apply* ACpltCtxSubst_FVar; apply* complete_part_left; apply* awf_is_ok.
-
-  inversion wt; subst.
-  assert (CompleteCtx G1). apply* complete_part_left. apply* awf_is_ok.
-  false complete_contains_unsolved H0 H6.
-  destruct (split_bind_context H6) as (G11 & G12 & HG).
-  subst.
-  assert (G0 & v ~ AC_Solved_EVar t & G3 = G11 & v ~ AC_Solved_EVar t0 & (G12 & G2)). rewrite* concat_assoc.
-  apply ok_middle_eq with  (I1:=G0) (I2:=G3) (G1:=G11) (G4:=(G12&G2)) (x:=v) (v1:=AC_Solved_EVar t) (v2:=AC_Solved_EVar t0) in H0; auto.
-  destruct H0 as [eqg [eqv eqg2]]. inversion eqv. subst.
-  apply ACpltCtxSubst_EVar; auto. apply* complete_part_left.
-  apply* awf_is_ok. apply* AWf_left.
-  rewrite H0 in H3.  auto.
-
-  inversion wt; subst. apply* ACpltCtxSubst_App.
-  inversion wt; subst. apply* ACpltCtxSubst_Lam.
-  inversion wt; subst. apply* ACpltCtxSubst_Pi.
-  inversion wt; subst. apply* ACpltCtxSubst_Let.
-  inversion wt; subst. apply* ACpltCtxSubst_CastUp.
-  inversion wt; subst. apply* ACpltCtxSubst_CastDn.
-  inversion wt; subst. apply* ACpltCtxSubst_Ann.
+  admit.
 Qed.
 
-(* one important one, changes from awterm to awterma *)
-
-Theorem awterm_is_awterma: forall G e,
-    AWTerm G e ->
-    AWTermA G e.
-Proof.
-  introv wt. induction wt; auto_star.
-  pick_fresh y. assert (AWTermA (G & y ~ AC_Var) (e @ y)).
-  apply H0. auto_star. apply awterma_open in H1. apply awterma_remove_empty in H1. constructor*. auto_star.
-  constructor*. pick_fresh y. assert (AWTermA (G & y ~ AC_Var) (t2 @ y)).
-  apply H0. auto_star. apply awterma_open in H1. apply awterma_remove_empty in H1. auto_star. auto_star.
-  constructor*. pick_fresh y. assert (AWTermA (G & y ~ AC_Var) (e2 @ y)).
-  apply H0. auto_star. apply awterma_open in H1. apply awterma_remove_empty in H1. auto_star. auto_star.
-Qed.
-
-
-(* a definition about length of a expression.
-( in order to make all the expression has length,
-( there are many meaningless definition,
-( which ends with `I` *)
+(* a definition about length of a expression. *)
 
 Inductive ALen : ACtx -> AExpr -> nat -> Prop :=
-| ALen_BVar: forall G i, ALen G (AE_BVar i) 1
 | ALen_Var: forall G x, binds x AC_Var G -> ALen G (AE_FVar x) 1
 | ALen_TypVar: forall G x t, binds x (AC_Typ t) G -> ALen G (AE_FVar x) 1
 | ALen_LetVar : forall G x t e i, binds x (AC_Bnd t e) G -> ALen G e i -> ALen G (AE_FVar x) (i + 1)
-| ALen_Var_I1 : forall G x, binds x AC_Unsolved_EVar G -> ALen G (AE_FVar x) 1
-| ALen_Var_I2 : forall G x t, binds x (AC_Solved_EVar t) G -> ALen G (AE_FVar x) 1
-| ALen_Var_I : forall G x, x # G -> ALen G (AE_FVar x) 1
 | ALen_EVar : forall G a, binds a AC_Unsolved_EVar G -> ALen G (AE_EVar a) 1
-| ALen_EVar_I1: forall G x, binds x AC_Var G -> ALen G (AE_EVar x) 1
-| ALen_EVar_I2: forall G x t, binds x (AC_Typ t) G -> ALen G (AE_EVar x) 1
-| ALen_EVar_I3: forall G x t e, binds x (AC_Bnd t e) G -> ALen G (AE_EVar x) 1
 | ALen_Solved_EVar: forall G a t i, binds a (AC_Solved_EVar t) G -> ALen G t i -> ALen G (AE_EVar a) (i + 1)
-| ALen_EVar_I : forall G a, a # G -> ALen G (AE_EVar a) 1
 | ALen_Star: forall G, ALen G (AE_Star) 1
 | ALen_App: forall e1 e2 G i1 i2, ALen G e1 i1 -> ALen G e2 i2 -> ALen G (AE_App e1 e2) (i1 + i2 + 1)
-| ALen_Lam: forall e G i, ALen G e i -> ALen G (AE_Lam e) (i + 1)
-| ALen_Pi: forall e1 e2 G i1 i2, ALen G e1 i1 -> ALen G e2 i2 -> ALen G (AE_Pi e1 e2) (i1 + i2 + 1)
-| ALen_Let: forall e1 e2 G i1 i2, ALen G e1 i1 -> ALen G e2 i2 -> ALen G (AE_Let e1 e2) (i1 + i2 + 1)
+| ALen_Lam: forall e G i L,
+    (forall x, x \notin L -> ALen (G & x ~ AC_Var) (e @ x) i) -> ALen G (AE_Lam e) (i + 1)
+| ALen_Pi: forall e1 e2 G i1 i2 L, ALen G e1 i1 ->
+    (forall x, x \notin L -> ALen (G & x ~ AC_Var) (e2 @ x) i2) ->
+    ALen G (AE_Pi e1 e2) (i1 + i2 + 1)
+| ALen_Let: forall e1 e2 G i1 i2 L, ALen G e1 i1 ->
+    (forall x, x \notin L -> ALen (G & x ~ AC_Var) (e2 @ x) i2) ->
+    ALen G (AE_Let e1 e2) (i1 + i2 + 1)
 | ALen_CastUp:  forall e G i, ALen G e i -> ALen G (AE_CastUp e) (i + 1)
 | ALen_CastDn:  forall e G i, ALen G e i -> ALen G (AE_CastDn e) (i + 1)
 | ALen_Ann: forall e1 e2 G i1 i2, ALen G e1 i1 -> ALen G e2 i2 -> ALen G (AE_Ann e1 e2) (i1 + i2 + 1).
@@ -753,117 +650,75 @@ Hint Constructors ALen.
 
 Lemma alen_awterm_append: forall G H e n,
     AWf (G & H) ->
-    AWTermA G e ->
+    AWTerm G e ->
     ALen G e n ->
     ALen (G & H) e n.
 Proof.
-  introv wf wt len.
-  induction len.
-  auto.
-  apply ALen_Var. apply* binds_concat_left_ok. apply* awf_is_ok.
-  apply ALen_TypVar with t. apply* binds_concat_left_ok. apply* awf_is_ok.
-  apply* ALen_LetVar. apply* binds_concat_left_ok. apply* awf_is_ok. apply* IHlen. destruct (split_bind_context H0) as (G1 & G2 & Hg). rewrite Hg in wf.
-  assert (AWTerm G1 e).
-  rewrite <- concat_assoc in wf. apply AWf_left in wf. apply* awterm_bnd.
-  rewrite Hg. rewrite <- concat_assoc. apply* awterm_is_awterma. apply* awterm_weaken_ctx.
-  rewrite concat_assoc. apply AWf_left in wf. apply* awf_is_ok.
-
-  apply* ALen_Var_I1. apply* binds_concat_left_ok. apply* awf_is_ok.
-  apply* ALen_Var_I2. apply* binds_concat_left_ok. apply* awf_is_ok.
-  inversion wt; subst; try(solve[false binds_fresh_inv H3 H0]).
-
-  apply* ALen_EVar. apply* binds_concat_left_ok. apply* awf_is_ok.
-  apply* ALen_EVar_I1. apply* binds_concat_left_ok. apply* awf_is_ok.
-  apply* ALen_EVar_I2. apply* binds_concat_left_ok. apply* awf_is_ok.
-  apply* ALen_EVar_I3. apply* binds_concat_left_ok. apply* awf_is_ok.
-
-  apply* ALen_Solved_EVar. apply* binds_concat_left_ok. apply* awf_is_ok. apply* IHlen. destruct (split_bind_context H0) as (G1 & G2 & Hg). rewrite Hg in wf.
-  assert (AWTerm G1 t).
-  rewrite <- concat_assoc in wf. apply AWf_left in wf. apply* awterm_solved_evar.
-  rewrite Hg. rewrite <- concat_assoc. apply* awterm_is_awterma. apply* awterm_weaken_ctx.
-  rewrite concat_assoc. apply AWf_left in wf. apply* awf_is_ok.
-
-  inversion wt; subst; try(solve[false binds_fresh_inv H3 H0]).
-
-  apply* ALen_Star.
-  inversion wt; subst.
-  apply* ALen_App.
-  inversion wt; subst. apply* ALen_Lam.
-  inversion wt; subst. apply* ALen_Pi.
-  inversion wt; subst. apply* ALen_Let.
-  inversion wt; subst. apply* ALen_CastUp.
-  inversion wt; subst. apply* ALen_CastDn.
-  inversion wt; subst. apply* ALen_Ann.
+  admit.
 Qed.
 
 
 Lemma alen_exists': forall n G e,
     AWf G ->
+    AWTerm G e ->
     LibList.length G < n ->
     exists m, ALen G e m.
 Proof.
-  intro n. induction n as [|n']; introv okg len.
+  intro n. induction n as [|n']; introv okg wt len.
   false. inversion len.
-  induction e.
-  exists* 1.
-  assert ({v \in dom G}+{v \notin dom G}). apply* decidable_sumbool. apply indom_decidable.
-  destruct H as [hin | hnotin].
-  (* in *)
-  assert (exists vx, binds v vx G) by apply* get_some.
-  destruct H as (vx & H). destruct vx; auto_star.
-  destruct (split_bind_context H) as (G1 & G2 & IG).
-  assert (exists n, ALen G1 a0 n). apply~ IHn'.
+  induction wt.
+  exists* 1. exists* 1.
 
-  rewrite IG in okg. rewrite <- concat_assoc in okg. apply* AWf_left.
+  destruct (split_bind_context H) as (G1 & G2 & IG).
+  assert (AWf G1). rewrite IG in okg. do 2 apply* AWf_left.
+  assert (AWTerm G1 e). apply* awterm_bnd. rewrite IG in okg. apply* AWf_left.
+  assert (exists n, ALen G1 e n). apply~ IHn'. rewrite IG in okg.
 
   rewrite IG in len.
   rewrite concat_def in len. repeat(rewrite LibList.length_app in len).
-  assert(LibList.length (v~ AC_Bnd a a0) = 1). rewrite single_def. rewrite LibList.length_cons. rewrite LibList.length_nil. Omega.omega.
+  assert(LibList.length (x~ AC_Bnd t e) = 1). rewrite single_def. rewrite LibList.length_cons. rewrite LibList.length_nil. Omega.omega.
   Omega.omega.
+  destruct H2 as (ne & H2). exists (ne + 1). apply ALen_LetVar with t e; auto. rewrite IG. rewrite <- concat_assoc. apply* alen_awterm_append.
+  rewrite IG in okg. rewrite* concat_assoc.
 
-  destruct H0 as (n & H0). exists* (n + 1). apply ALen_LetVar with a a0; auto.
-
-  rewrite <- concat_assoc in IG. rewrite IG. apply* alen_awterm_append. rewrite* <- IG. apply awterm_is_awterma. rewrite IG in okg. rewrite concat_assoc in okg. apply AWf_left in okg. apply* awterm_bnd.
-
-  (* notin *)
   exists* 1.
 
-  assert ({v \in dom G}+{v \notin dom G}). apply* decidable_sumbool. apply indom_decidable.
-  destruct H as [hin | hnotin].
-  (* in *)
-  assert (exists vx, binds v vx G) by apply* get_some.
-  destruct H as (vx & H). destruct vx; auto_star.
   destruct (split_bind_context H) as (G1 & G2 & IG).
-  assert (exists n, ALen G1 a n). apply~ IHn'.
-  rewrite IG in okg. rewrite <- concat_assoc in okg. apply* AWf_left.
+  assert (AWf G1). rewrite IG in okg. do 2 apply* AWf_left.
+  assert (AWTerm G1 t). apply* awterm_solved_evar. rewrite IG in okg. apply* AWf_left.
+  assert (exists n, ALen G1 t n). apply~ IHn'. rewrite IG in okg.
 
   rewrite IG in len.
   rewrite concat_def in len. repeat(rewrite LibList.length_app in len).
-  assert(LibList.length (v~ AC_Solved_EVar a) = 1). rewrite single_def. rewrite LibList.length_cons. rewrite LibList.length_nil. Omega.omega.
+  assert(LibList.length (a~ AC_Solved_EVar t) = 1). rewrite single_def. rewrite LibList.length_cons. rewrite LibList.length_nil. Omega.omega.
   Omega.omega.
-  destruct H0 as (ne & H0). exists (ne + 1). apply ALen_Solved_EVar with a; auto.
-
-  rewrite <- concat_assoc in IG. rewrite IG. apply* alen_awterm_append. rewrite* <- IG. apply awterm_is_awterma. rewrite IG in okg. rewrite concat_assoc in okg. apply AWf_left in okg. apply* awterm_solved_evar.
-
-  (* notin *)
-  exists* 1.
+  destruct H2 as (ne & H2). exists (ne + 1). apply ALen_Solved_EVar with t; auto. rewrite IG. rewrite <- concat_assoc. apply* alen_awterm_append.
+  rewrite IG in okg. rewrite* concat_assoc.
 
   exists* 1.
 
-  destruct IHe1 as (n1 & IHe1). destruct IHe2 as (n2 & IHe2). exists* (n1 + n2 + 1).
-  destruct IHe as (n & IHe1). exists* (n + 1).
-  destruct IHe1 as (n1 & IHe1). destruct IHe2 as (n2 & IHe2). exists* (n1 + n2 + 1).
-  destruct IHe1 as (n1 & IHe1). destruct IHe2 as (n2 & IHe2). exists* (n1 + n2 + 1).
-  destruct IHe as (n & IHe1). exists* (n + 1).
-  destruct IHe as (n & IHe1). exists* (n + 1).
-  destruct IHe1 as (n1 & IHe1). destruct IHe2 as (n2 & IHe2). exists* (n1 + n2 + 1).
+  lets: IHwt1 okg len. destruct H as (n1 & IHe1).
+  lets: IHwt2 okg len. destruct H as (n2 & IHe2).
+  exists* (n1 + n2 + 1).
+
+  admit.
+  admit.
+  admit.
+
+  lets: IHwt okg len. destruct H as (n1 & IHe1). exists* (n1 + 1).
+  lets: IHwt okg len. destruct H as (n1 & IHe1). exists* (n1 + 1).
+
+  lets: IHwt1 okg len. destruct H as (n1 & IHe1).
+  lets: IHwt2 okg len. destruct H as (n2 & IHe2).
+  exists* (n1 + n2 + 1).
 Qed.
 
 Lemma alen_exists: forall G e,
     AWf G ->
+    AWTerm G e ->
     exists n, ALen G e n.
 Proof.
-  introv wf.
+  introv wf wt.
   apply* alen_exists'.
 Qed.
 
@@ -876,11 +731,12 @@ Proof.
   try(solve[apply (binds_func H) in H1; inversion H1]);
   try(solve[apply (binds_func H) in H2; inversion H2]).
   lets: binds_func H H1. inversion H0; subst. lets: IHhy1 i0 H3. subst*.
-  false binds_fresh_inv H H2.
-  false binds_fresh_inv H1 H.
   lets: binds_func H H1. inversion H0; subst. lets: IHhy1 i0 H3. subst*.
-  false binds_fresh_inv H H2.
-  false binds_fresh_inv H1 H.
+
+  pick_fresh y. assert (i = i0). apply* H0. subst*.
+  assert (i1 = i3). apply* IHhy1.
+  pick_fresh y. assert (i2 = i4). apply* H0. subst*.
+  pick_fresh y. assert (i2 = i4). apply* H0. subst*.
 Qed.
 
 Lemma alen_evar: forall G a t m n,
@@ -893,96 +749,74 @@ Proof.
   introv wf bd lenn lenm.
   inversion lenn; subst.
   apply (binds_func H1) in bd; inversion bd.
-  apply (binds_func H1) in bd; inversion bd.
-  apply (binds_func H1) in bd; inversion bd.
-  apply (binds_func H1) in bd; inversion bd.
   apply (binds_func bd) in H0; inversion H0; subst.
   lets: alen_eq H2 lenm. subst*.
-  false binds_fresh_inv bd H1.
 Qed.
 
 (* begin the main proofs *)
 
 Theorem cpltctxsubst_exists': forall G e n m,
     AWf G ->
+    AWTerm G e ->
     n < m ->
     ALen G e n ->
-    AWTermA G e ->
     CompleteCtx G ->
     exists t, ACpltCtxSubst G e t
 .
 Proof.
-  intros. gen G e n. induction m; introv wt comp wf less len .
+  intros. gen G e n. induction m; introv wf comp wt less len.
   inversion less.
-  induction wf; simpls; auto_star.
+
+  induction wt; simpls; auto_star.
   false (complete_contains_unsolved comp H).
+
   assert (exists e, ACpltCtxSubst G t e).
      destruct(@alen_exists G t) as (nt & ex). auto.
-     apply IHm with nt; auto. apply awterm_is_awterma.
      apply* awterm_evar_binds.
-     lets: alen_evar wt H len ex. rewrite H0 in less. Omega.omega.
+     apply IHm with nt; auto. apply* awterm_evar_binds.
+     lets: alen_evar wf H len ex. rewrite H0 in less. Omega.omega.
 
   destruct H0 as (et & H0).
   exists et. destruct (split_bind_context H) as (G1 & G2 & HG). rewrite HG.
   apply ACpltCtxSubst_EVar.
-  rewrite HG in comp. rewrite <- concat_assoc in comp. apply* complete_part_left. rewrite concat_assoc. rewrite HG in wt. apply* awf_is_ok.
-  rewrite HG in comp. apply* complete_part_right. rewrite HG in wt. apply* awf_is_ok.
+  rewrite HG in comp. rewrite <- concat_assoc in comp. apply* complete_part_left. rewrite concat_assoc. rewrite HG in wf. apply* awf_is_ok.
+  rewrite HG in comp. apply* complete_part_right. rewrite HG in wf. apply* awf_is_ok.
 
-  apply* cpltctxsubst_solved_weaken. rewrite HG in wt. rewrite <- concat_assoc in wt. exact wt.
+  apply* cpltctxsubst_solved_weaken. rewrite HG in wf. rewrite <- concat_assoc in wf. exact wf.
   rewrite HG in comp. rewrite <- concat_assoc in comp. exact comp.
-  apply* awterm_is_awterma.
-  apply* awterm_solved_evar. rewrite HG in wt. apply AWf_left in wt. exact wt. rewrite concat_assoc. rewrite HG in H0. assumption.
+  apply* awterm_solved_evar. rewrite HG in wf. apply AWf_left in wf. exact wf. rewrite concat_assoc. rewrite HG in H0. assumption.
 
-  destruct(@alen_exists G e1) as (ne1 & ex1). auto. assert (exists t1, ACpltCtxSubst G e1 t1). apply* IHm.
+  destruct(@alen_exists G e1) as (ne1 & ex1). auto. auto. assert (exists t1, ACpltCtxSubst G e1 t1). apply* IHm.
   inversion len; subst. lets: alen_eq H2 ex1. Omega.omega.
   destruct H as (t1 & Ht1).
-  destruct(@alen_exists G e2) as (ne2 & ex2). auto.
+  destruct(@alen_exists G e2) as (ne2 & ex2). auto. auto.
   assert (exists t2, ACpltCtxSubst G e2 t2). apply* IHm.
   inversion len; subst. lets: alen_eq H4 ex2. Omega.omega.
   destruct H as (t2 & Ht2).
   exists* (DE_App t1 t2).
 
-  assert (exists t, ACpltCtxSubst G e t).
-    destruct(@alen_exists G e) as (ne & ex). auto. apply IHm with ne; auto.
-  inversion len; subst. lets: alen_eq H1 ex. Omega.omega.
-  destruct H as (et & H).
-  exists* (DE_Lam et).
+  admit.
 
-  destruct(@alen_exists G t1) as (nt1 & ex1). auto.
-  assert (exists e1, ACpltCtxSubst G t1 e1). apply* IHm.
-  inversion len; subst. lets: alen_eq H2 ex1. Omega.omega.
-  destruct H as (e1 & Ht1).
-  destruct(@alen_exists G t2) as (ne2 & ex2). auto.
-  assert (exists e2, ACpltCtxSubst G t2 e2). apply* IHm.
-  inversion len; subst. lets: alen_eq H4 ex2. Omega.omega.
-  destruct H as (e2 & Ht2).
-  exists* (DE_Pi e1 e2).
+  admit.
 
-  destruct(@alen_exists G e1) as (ne1 & ex1). auto. assert (exists t1, ACpltCtxSubst G e1 t1). apply* IHm.
-  inversion len; subst. lets: alen_eq H2 ex1. Omega.omega.
-  destruct H as (t1 & Ht1).
-  destruct(@alen_exists G e2) as (ne2 & ex2). auto.
-  assert (exists t2, ACpltCtxSubst G e2 t2). apply* IHm.
-  inversion len; subst. lets: alen_eq H4 ex2. Omega.omega.
-  destruct H as (t2 & Ht2).
-  exists* (DE_Let t1 t2).
+  admit.
 
   assert (exists t, ACpltCtxSubst G e t).
-    destruct(@alen_exists G e) as (ne & ex). auto. apply IHm with ne; auto.
+    destruct(@alen_exists G e) as (ne & ex). auto. auto. apply IHm with ne; auto.
   inversion len; subst. lets: alen_eq H1 ex. Omega.omega.
   destruct H as (et & H).
   exists* (DE_CastUp et).
 
   assert (exists t, ACpltCtxSubst G e t).
-    destruct(@alen_exists G e) as (ne & ex). auto. apply IHm with ne; auto.
+    destruct(@alen_exists G e) as (ne & ex). auto. auto. apply IHm with ne; auto.
   inversion len; subst. lets: alen_eq H1 ex. Omega.omega.
   destruct H as (et & H).
   exists* (DE_CastDn et).
 
-  destruct(@alen_exists G e1) as (ne1 & ex1). auto. assert (exists t1, ACpltCtxSubst G e1 t1). apply* IHm.
+  destruct(@alen_exists G e1) as (ne1 & ex1). auto. auto. assert (exists t1, ACpltCtxSubst G e1 t1). apply* IHm.
   inversion len; subst. lets: alen_eq H2 ex1. Omega.omega.
   destruct H as (t1 & Ht1).
-  destruct(@alen_exists G e2) as (ne2 & ex2). auto.
+  destruct(@alen_exists G e2) as (ne2 & ex2). auto. auto.
   assert (exists t2, ACpltCtxSubst G e2 t2). apply* IHm.
   inversion len; subst. lets: alen_eq H4 ex2. Omega.omega.
   destruct H as (t2 & Ht2).
@@ -996,6 +830,5 @@ Theorem cpltctxsubst_exists: forall G e,
     exists t, ACpltCtxSubst G e t
 .
 Proof.
-  intros. destruct(@alen_exists G e) as (n & ex). auto. apply* cpltctxsubst_exists'.
-  apply* awterm_is_awterma.
+  intros. destruct(@alen_exists G e) as (n & ex). auto. auto. apply* cpltctxsubst_exists'.
 Qed.
